\begin{dmath*}
Omega = 1
\end{dmath*}
\begin{dmath*}
YoverC = \frac{1.0}{{\bar{C_K}}+{\bar{C_R}}}
\end{dmath*}
\begin{dmath*}
InvoverC = \frac{{{\frac{\bar{I}}{\bar{Y}}}}}{{\bar{C_K}}+{\bar{C_R}}}
\end{dmath*}
\begin{dmath*}
psi\_n\_ya = \frac{1+{{\phi}}}{{{\alpha}}+{{\phi}}+{{\sigma}}\, {YoverC_{t}}\, \left(1-{{\alpha}}\right)}
\end{dmath*}
\begin{dmath*}
lambda\_gali = \frac{\left(1-{{\theta}}\right)\, \left(1-{{\theta}}\, {{\beta}}\right)}{{{\theta}}}\, {Omega_{t}}
\end{dmath*}
\begin{dmath*}
kappa = {lambda\_gali_{t}}\, \left({{\sigma}}\, {YoverC_{t}}+\frac{{{\phi}}+{{\alpha}}}{1-{{\alpha}}}\right)
\end{dmath*}
% Equation 1
\begin{dmath}
{{\pi}_{t}}={{\beta}}\, {{\pi}_{t+1}}+{kappa_{t}}\, {{\tilde y}_{t}}
\end{dmath}
% Equation 2
\begin{dmath}
{{w_r}_{t}}=\frac{{{\sigma}}\, \left({\bar{C_R}}\, {{c_R}_{t}}+{\bar{C_K}}\, {{c_K}_{t}}\right)}{{\bar{C_K}}+{\bar{C_R}}}+{{\phi}}\, {{n}_{t}}
\end{dmath}
% Equation 3
\begin{dmath}
{{n_R}_{t}}={{n_K}_{t}}
\end{dmath}
% Equation 4
\begin{dmath}
{{c_R}_{t}}={{c_R}_{t+1}}-\frac{1}{{{\sigma}}}\, \left({{i}_{t}}-{{\pi}_{t+1}}\right)
\end{dmath}
% Equation 5
\begin{dmath}
{{c_K}_{t}}\, \left(1-{{\Lambda}}\, \left(1-{{\beta}}\right)\right)={{w_r}_{t}}+{{n_K}_{t}}-{{\Lambda}}\, \left({{i}_{t-1}}-{{\pi}_{t}}-{{r^r}_{t-1}}\right)-{{\beta}}\, {{\Lambda}}\, {{r^r}_{t}}
\end{dmath}
% Equation 6
\begin{dmath}
{{y}_{t}}={\bar{C_R}}\, {{c_R}_{t}}+{\bar{C_K}}\, {{c_K}_{t}}+{{\frac{\bar{I}}{\bar{Y}}}}\, {{i_R}_{t}}
\end{dmath}
% Equation 7
\begin{dmath}
{{n}_{t}}={{n_R}_{t}}\, {\bar{N_R}}+{{n_K}_{t}}\, {\bar{N_K}}
\end{dmath}
% Equation 8
\begin{dmath}
{{c}_{t}}=\frac{{\bar{C_R}}\, {{c_R}_{t}}+{\bar{C_K}}\, {{c_K}_{t}}}{{\bar{C_K}}+{\bar{C_R}}}
\end{dmath}
% Equation 9
\begin{dmath}
{{i_R}_{t}}\, {{\delta}}={{k}_{t}}-\left(1-{{\delta}}\right)\, {{k}_{t-1}}
\end{dmath}
% Equation 10
\begin{dmath}
{{q}_{t}}={{\psi_c}}\, \left({{k}_{t}}-{{k}_{t-1}}\right)
\end{dmath}
% Equation 11
\begin{dmath}
{{r^r}_{t}}+{{q}_{t}}={{\beta}}\, \left(1-{{\delta}}\right)\, {{q}_{t+1}}+\left(1-{{\beta}}\, \left(1-{{\delta}}\right)\right)\, \left({{w_r}_{t+1}}+{{n}_{t+1}}-{{k}_{t}}\right)
\end{dmath}
% Equation 12
\begin{dmath}
{{i}_{t}}={{\pi}_{t}}\, {{\phi_{\pi}}}+{{\tilde y}_{t}}\, {{\phi_{y}}}+{{\nu}_{t}}
\end{dmath}
% Equation 13
\begin{dmath}
{{r^r}_{t}}={{i}_{t}}-{{\pi}_{t+1}}
\end{dmath}
% Equation 14
\begin{dmath}
{{y^{nat}}_{t}}={psi\_n\_ya_{t}}\, \left({{a}_{t}}+{{\alpha}}\, {{k}_{t-1}}\right)+{{i_R}_{t}}\, \frac{{{\sigma}}\, \left(1-{{\alpha}}\right)\, {InvoverC_{t}}}{{{\alpha}}+{{\phi}}+{YoverC_{t}}\, {{\sigma}}\, \left(1-{{\alpha}}\right)}
\end{dmath}
% Equation 15
\begin{dmath}
{{\tilde y}_{t}}={{y}_{t}}-{{y^{nat}}_{t}}
\end{dmath}
% Equation 16
\begin{dmath}
{{\nu}_{t}}={{\rho_{\nu}}}\, {{\nu}_{t-1}}+{{\varepsilon_\nu}_{t}}
\end{dmath}
% Equation 17
\begin{dmath}
{{a}_{t}}=0
\end{dmath}
% Equation 18
\begin{dmath}
{{y}_{t}}={{\alpha}}\, {{k}_{t-1}}+{{a}_{t}}+\left(1-{{\alpha}}\right)\, {{n}_{t}}
\end{dmath}
