\begin{dmath*}
Omega = \frac{1-{{\alpha}}}{1-{{\alpha}}+{{\alpha}}\, {{\epsilon}}}
\end{dmath*}
\begin{dmath*}
psi\_n\_ya = \frac{1+{{\phi}}}{{{\alpha}}+{{\phi}}+\left(1-{{\alpha}}\right)\, {{\sigma}}}
\end{dmath*}
\begin{dmath*}
lambda = \frac{\left(1-{{\theta}}\right)\, \left(1-{{\theta}}\, {{\beta}}\right)}{{{\theta}}}\, {Omega_{t}}
\end{dmath*}
\begin{dmath*}
kappa = {lambda_{t}}\, \left({{\sigma}}+\frac{{{\alpha}}+{{\phi}}}{1-{{\alpha}}}\right)
\end{dmath*}
% Equation 1
\begin{dmath}
{{\pi}_{t}}={{\beta}}\, {{\pi}_{t+1}}+{kappa_{t}}\, {{\tilde y}_{t}}
\end{dmath}
% Equation 2
\begin{dmath}
{{\tilde y}_{t}}=\frac{\left(-1\right)}{{{\sigma}}}\, \left({{i}_{t}}-{{\pi}_{t+1}}-{{r^{nat}}_{t}}\right)+{{\tilde y}_{t+1}}
\end{dmath}
% Equation 3
\begin{dmath}
{{i}_{t}}={{\pi}_{t}}\, {{\phi_{\pi}}}+{{\tilde y}_{t}}\, {{\phi_{y}}}+{{\nu}_{t}}
\end{dmath}
% Equation 4
\begin{dmath}
{{r^{nat}}_{t}}={{\sigma}}\, {psi\_n\_ya_{t}}\, \left({{a}_{t+1}}-{{a}_{t}}\right)
\end{dmath}
% Equation 5
\begin{dmath}
{{r^r}_{t}}={{i}_{t}}-{{\pi}_{t+1}}
\end{dmath}
% Equation 6
\begin{dmath}
{{y^{nat}}_{t}}={psi\_n\_ya_{t}}\, {{a}_{t}}
\end{dmath}
% Equation 7
\begin{dmath}
{{\tilde y}_{t}}={{y}_{t}}-{{y^{nat}}_{t}}
\end{dmath}
% Equation 8
\begin{dmath}
{{\nu}_{t}}={{\rho_{\nu}}}\, {{\nu}_{t-1}}+{{\varepsilon_\nu}_{t}}
\end{dmath}
% Equation 9
\begin{dmath}
{{a}_{t}}=0
\end{dmath}
% Equation 10
\begin{dmath}
{{y}_{t}}={{a}_{t}}+\left(1-{{\alpha}}\right)\, {{n}_{t}}
\end{dmath}
